Update VectorSpace.thy
Connected with Linear_Algebra_On_With

VectorSpace.thy
@@ -1,21 +1,103 @@
 theory VectorSpace
-  imports Main HOL.Real
+  imports Main HOL.Real "HOL-Types_To_Sets.Linear_Algebra_On_With"
+
 begin
 
 locale vector_space_with_domain =
   fixes dom :: "'a set"
-    and add :: "'a \<Rightarrow> 'a \<Rightarrow> 'a"      
+    and add :: "'a ⇒ 'a ⇒ 'a"      
     and zero :: "'a"
-    and smult :: "real \<Rightarrow> 'a \<Rightarrow> 'a"   
-  assumes add_closed: "\<lbrakk>x \<in> dom; y \<in> dom\<rbrakk> \<Longrightarrow> add x y \<in> dom" 
-    and zero_in_dom: "zero \<in> dom"      
-    and add_assoc: "\<lbrakk>x \<in> dom; y \<in> dom; z\<in> dom\<rbrakk> \<Longrightarrow>add (add x y) z = add x (add y z)"
-    and add_comm: "\<lbrakk>x \<in> dom; y \<in> dom\<rbrakk> \<Longrightarrow> add x y = add y x"
-    and add_zero: "\<lbrakk>x \<in> dom\<rbrakk> \<Longrightarrow> add x zero = x"
-    and add_inv: "x \<in> dom \<Longrightarrow> \<exists>y \<in> dom. add x y = zero"
-    and smult_closed: "\<lbrakk>x \<in> dom\<rbrakk> \<Longrightarrow> smult a x \<in> dom"
-    and smult_distr_sadd: "\<lbrakk>x \<in> dom\<rbrakk> \<Longrightarrow>smult (a + b) x = add (smult a x) (smult b x)"
-    and smult_assoc: "\<lbrakk>x \<in> dom\<rbrakk> \<Longrightarrow> smult a  (smult b x) = smult (a * b)  x"
-    and smult_one: "\<lbrakk>x \<in> dom\<rbrakk> \<Longrightarrow> smult 1 x = x" 
+    and smult :: "real ⇒ 'a ⇒ 'a"   
+  assumes add_closed: "⟦x ∈ dom; y ∈ dom⟧ ⟹ add x y ∈ dom" 
+    and zero_in_dom: "zero ∈ dom"      
+    and add_assoc: "⟦x ∈ dom; y ∈ dom; z∈ dom⟧ ⟹add (add x y) z = add x (add y z)"
+    and add_comm: "⟦x ∈ dom; y ∈ dom⟧ ⟹ add x y = add y x"
+    and add_zero: "⟦x ∈ dom⟧ ⟹ add x zero = x"
+    and add_inv: "x ∈ dom ⟹ ∃y ∈ dom. add x y = zero"
+    and smult_closed: "⟦x ∈ dom⟧ ⟹ smult a x ∈ dom"
+    and smult_distr_sadd: "⟦x ∈ dom⟧ ⟹smult (a + b) x = add (smult a x) (smult b x)"
+    and smult_assoc: "⟦x ∈ dom⟧ ⟹ smult a  (smult b x) = smult (a * b)  x"
+    and smult_one: "⟦x ∈ dom⟧ ⟹ smult 1 x = x" 
+    and smult_distr_sadd2: "⟦x ∈ dom; y∈dom⟧ ⟹ smult a (add x y) = add (smult a x) (smult a y)"
+
+begin
+
+lemma inv_unique:
+  assumes "a∈dom" "z1∈dom" "z2∈dom"
+      "add a z1 = zero"
+      "add a z2 = zero"
+    shows "z1=z2"
+  by (metis add_assoc add_comm add_zero assms)
+
+definition inv::"'a⇒'a" where 
+    "inv a = (if a∈dom then (THE z. (z∈dom ∧ add a z = zero)) else undefined)"
+
+definition minus::"'a⇒'a⇒'a" where
+    "minus a b = (if a∈dom ∧ b∈dom then add a (inv b) else undefined)"
+
+lemma module_on_with_is_this:
+  shows "module_on_with dom add minus inv zero smult"
+  unfolding module_on_with_def
+proof
+  show "ab_group_add_on_with dom add zero local.minus local.inv"
+    unfolding ab_group_add_on_with_def
+  proof
+    show "comm_monoid_add_on_with dom add zero"
+      by (smt (verit, del_insts) ab_semigroup_add_on_with_Ball_def add_assoc add_closed add_comm add_zero comm_monoid_add_on_with_Ball_def semigroup_add_on_with_def zero_in_dom)
+    next
+    show "ab_group_add_on_with_axioms dom add zero local.minus local.inv"
+      unfolding ab_group_add_on_with_axioms_def
+    proof
+      show "∀a. a ∈ dom ⟶ add (local.inv a) a = zero"
+      proof-
+        {fix a 
+          assume "a∈dom"
+          obtain "z" where "z∈dom ∧ add z a = zero"
+            using ‹a ∈ dom› add_comm add_inv by blast
+          moreover have "local.inv a = z"
+            using ‹a ∈ dom› add_comm calculation inv_unique local.inv_def by auto
+          ultimately have " add (local.inv a) a = zero"
+          using `a∈dom`
+          by fastforce
+          
+      }
+      show ?thesis 
+        using ‹⋀aa. aa ∈ dom ⟹ add (local.inv aa) aa = zero› by blast
+    qed
+  next
+    show " (∀a b. a ∈ dom ⟶ b ∈ dom ⟶ local.minus a b = add a (local.inv b)) ∧
+    (∀a. a ∈ dom ⟶ local.inv a ∈ dom)"
+    proof
+      show "∀a b. a ∈ dom ⟶ b ∈ dom ⟶ local.minus a b = add a (local.inv b)"
+        using minus_def by auto
+    next
+      show "∀a. a ∈ dom ⟶ local.inv a ∈ dom"
+      proof-
+        {fix a 
+        assume "a∈dom"
+        have "local.inv a ∈dom"
+          by (smt (z3) ‹a ∈ dom› add_assoc add_comm add_inv add_zero local.inv_def theI')
+      }
+      show ?thesis 
+        using ‹⋀aa. aa ∈ dom ⟹ local.inv aa ∈ dom› by fastforce
+        qed
+      qed
+  qed  
+  qed
+next
+  show " ((∀a. ∀x∈dom. ∀y∈dom. smult a (add x y) = add (smult a x) (smult a y)) ∧
+     (∀a b. ∀x∈dom. smult (a + b) x = add (smult a x) (smult b x))) ∧
+    (∀a b. ∀x∈dom. smult a (smult b x) = smult (a * b) x) ∧
+    (∀x∈dom. smult 1 x = x) ∧ (∀a. ∀x∈dom. smult a x ∈ dom)"
+    using smult_one smult_distr_sadd smult_assoc smult_closed
+      smult_distr_sadd2
+    by auto
+qed
+
+lemma vector_space_on_with_is_this:
+  shows "vector_space_on_with dom add minus inv zero smult"
+  by (simp add: module_on_with_is_this vector_space_on_with_def)
+
+end
 
 end
